\documentclass{article}
\usepackage{amsmath}
\usepackage{mathrsfs}
\usepackage{extarrows}
\usepackage{array}
\usepackage{booktabs}

\title{Control Theory}
\author{Tristan Slater}

\begin{document}
    \maketitle

    \section{Systems}

    \subsection{Linearity}

    \begin{equation}
        f(ax + by) = af(x) + bf(y)
    \end{equation}

    \subsection{Time-Invariance}

    System is not directly dependent on time: \begin{equation}
        y(t) = F(x(t), t) = F(x(t))
    \end{equation}

    This also means that any shift to time in input translates to the same shift in the output.

    \begin{equation}
        x(t + \delta) \xlongrightarrow{F} y(t + \delta)
    \end{equation}

    \section{Convolution}

    \begin{equation}
        (f * g)(t) = \int_{-\infty}^\infty{f(\tau)g(t - \tau)\ d\tau}
    \end{equation}

    \section{Laplace Transform}

    \begin{equation}
        F(s) = \mathscr{L}\{f(t)\} = \int_0^\infty{e^{-st} f(t) dt}
    \end{equation}

    \begin{table}[h]
        \centering
        \caption{Laplace Lookup}
        $$\def\arraystretch{3}
        \begin{array}{>$l<$>{\displaystyle}c|>{\displaystyle}c}
            & f(t) = \mathscr{L}^{-1}\{F(s)\} & F(s) = \mathscr{L}\{f(t)\} \\
            \hline
            Multiplying by a Constant & af(at) & aF(s) \\
            Time Scaling & f(at) & \frac{1}{a}F\left(\frac{s}{a}\right) \\
            Frequency Scaling & \frac{1}{a}f\left(\frac{t}{a}\right) & F(as) \\
            Time Shifting & f(t - a)u(t - a) & e^{-at}F(s) \\
            Frequency Shifting & e^{at} f(t) & F(s - a) \\
            \hline
            Convolution & (f * g)(t) & F(s)G(s) = G(s)F(s) \\
            \hline
            & 1 & \frac{1}{s} \\
            & t^n & \frac{n!}{s^{n + 1}} \\
            & \sin{at} & \frac{a}{s^2 + a^2} \\
            & \cos{at} & \frac{s}{s^2 + a^2} \\
            & \sinh{at} & \frac{a}{s^2 - a^2} \\
            & \cosh{at} & \frac{s}{s^2 - a^2} \\
        \end{array}$$
    \end{table}

    \section{Transfer Functions}

    $$\begin{aligned}
        a_2\ddot{x} + a_1\dot{x} + a_0x &= b_2\ddot{y} + b_1\dot{y} + b_0y \\
        \mathscr{L}\{a_2\ddot{x} + a_1\dot{x} + a_0x\} &= \mathscr{L}\{b_2\ddot{y} + b_1\dot{y} + b_0y\} \\
        a_2s^2X(s) + a_1sX(s) + a_0X(s) &= b_2s^2Y(s) + b_1sY(S) + b_0Y(s) \\
        G(s) = \frac{Y(s)}{X(s)} &= \frac{b_2s^2 + b_1s + b_0}{a_2s^2 + a_1s + a_0} \\
    \end{aligned}$$

    Notes: \begin{itemize}
        \item All initial conditions are zero
        \item $X(s) \neq a_2s^2 + a_1s + a_0$
        \item $Y(s) \neq b_2s^2 + b_1s + b_0$
    \end{itemize}

    $$\begin{aligned}
        G(s) &= \frac{Y(s)}{X(s)} \\
        Y(s) &= G(s)X(s) \\
        \mathscr{L}^{-1}\{Y(s)\} &= \mathscr{L}^{-1}\{G(s)X(s)\} \\
        y(t) &= (g * x)(t) \\
        &= \int_{-\infty}^\infty{g(\tau)x(t - \tau)\ d\tau} \\
        &= \int_{-\infty}^\infty{x(\tau)g(t - \tau)\ d\tau} \\
    \end{aligned}$$

    \section{Impulse Response}

    $$\begin{aligned}
        Y(s) &= G(s) \\
        \mathscr{L}^{-1}\{Y(s)\} &= \mathscr{L}^{-1}\{G(s)\} \\
        y(t) &= g(t)
    \end{aligned}$$
\end{document}
