\documentclass{article}
\usepackage{amsmath}
\usepackage{mathrsfs}
\usepackage{extarrows}
\usepackage{array}
\usepackage{booktabs}

\title{Systems}
\author{Tristan Slater}

\begin{document}
    \maketitle

    \section{Properties}

    \subsection{Linearity}

    \begin{equation}
        f(ax + by) = af(x) + bf(y)
    \end{equation}

    \subsection{Time-Invariance}

    System is not directly dependent on time: \begin{equation}
        y(t) = F(x(t), t) = F(x(t))
    \end{equation}

    This also means that any shift to time in input translates to the same shift in the output.

    \begin{equation}
        x(t + \delta) \xlongrightarrow{F} y(t + \delta)
    \end{equation}

    \section{Convolution}

    \begin{equation}
        (f * g)(t) = \int_{-\infty}^\infty{f(\tau)g(t - \tau)\ d\tau}
    \end{equation}

    Properties: \begin{itemize}
        \item Commutative
    \end{itemize}

    \section{Transfer Functions}

    $$\begin{aligned}
        a_2\ddot{x} + a_1\dot{x} + a_0x &= b_2\ddot{y} + b_1\dot{y} + b_0y \\
        \mathscr{L}\{a_2\ddot{x} + a_1\dot{x} + a_0x\} &= \mathscr{L}\{b_2\ddot{y} + b_1\dot{y} + b_0y\} \\
        a_2s^2X(s) + a_1sX(s) + a_0X(s) &= b_2s^2Y(s) + b_1sY(S) + b_0Y(s) \\
        G(s) = \frac{Y(s)}{X(s)} &= \frac{b_2s^2 + b_1s + b_0}{a_2s^2 + a_1s + a_0} \\
    \end{aligned}$$

    Notes: \begin{itemize}
        \item All initial conditions are zero
        \item $X(s) \neq a_2s^2 + a_1s + a_0$
        \item $Y(s) \neq b_2s^2 + b_1s + b_0$
    \end{itemize}

    $$\begin{aligned}
        G(s) &= \frac{Y(s)}{X(s)} \\
        Y(s) &= G(s)X(s) \\
        \mathscr{L}^{-1}\{Y(s)\} &= \mathscr{L}^{-1}\{G(s)X(s)\} \\
        y(t) &= (g * x)(t) \\
        &= \int_{-\infty}^\infty{g(\tau)x(t - \tau)\ d\tau} \\
        &= \int_{-\infty}^\infty{x(\tau)g(t - \tau)\ d\tau} \\
    \end{aligned}$$

    \section{Impulse Response}

    $$\begin{aligned}
        Y(s) &= G(s) \\
        \mathscr{L}^{-1}\{Y(s)\} &= \mathscr{L}^{-1}\{G(s)\} \\
        y(t) &= g(t)
    \end{aligned}$$
\end{document}
